deps/poulet4/lib/Grammars/Binary.v
@@ -10,12 +10,10 @@ Import List.ListNotations.
 Open Scope list_scope.
 
 Definition binDigit : grammar nat := gsum [
-  glit "0" @ (fun _ => 0);
-  glit "1" @ (fun _ => 1)
+  glit true @ (fun _ => 0);
+  glit false @ (fun _ => 1)
 ].
 
 Definition gbin := gplus binDigit @ (fun ds => List.fold_left (fun a x => 2*a + x) ds 0).
-
-Check Vector.fold_left.
 
 Definition gbin_n (n: nat) := repeat n binDigit @ (fun ds => Vector.fold_left (fun a x => 2*a + x) 0 ds).
